Added proof

new/Ewflag_rid_map.fst
@@ -2,13 +2,16 @@ module Ewflag_rid_map
 
 module M = Map_extended
 module S = FStar.Set
+open SeqUtils
+open FStar.Seq
+open FStar.Ghost
 
 #set-options "--query_stats"
 let cf = (int * bool)
 
 // the concrete state type
 type concrete_st = M.t nat cf // (replica_id, ctr, flag) //replica ids are unique
- 
+
 let init_st : concrete_st = M.const (0, false)
 
 let sel (s:concrete_st) k = if M.contains s k then M.sel s k else (0, false)
@@ -41,11 +44,70 @@ type op_t = timestamp_t & (nat (*replica_id*) & app_op_t)
 
 let get_rid (_,(rid,_)) = rid
 
+type log = seq op_t
+
+let mem_rid (rid:nat) (l:log) =
+  exists e. mem e l /\ fst (snd e) = rid
+
+unfold
+let ( ++ ) (l1 l2:log) = Seq.append l1 l2
+
+unfold
+let mem_id (id:timestamp_t) (l:log) : bool =
+  mem_assoc_fst id l
+  
+unfold
+let distinct_ops (l:log) = distinct_assoc_fst l
+
+type st0 = concrete_st & erased log
+  
+let v_of (s:st0) : concrete_st = fst s
+let ops_of (s:st0) : GTot log = snd s
+
 // apply an operation to a state
 let do (s:concrete_st) (o:op_t) : concrete_st =
   match o with
   |(_, (rid, Enable)) -> M.upd s rid (fst (sel s rid) + 1, true) 
   |(_, (rid, Disable)) -> M.map_val (fun (c,f) -> (c, false)) s 
+
+let lem_do (a b:concrete_st) (op:op_t)
+   : Lemma (requires eq a b)
+           (ensures eq (do a op) (do b op)) = ()
+
+// applying a log of operations to a concrete state
+let rec apply_log (x:concrete_st) (l:log) : Tot concrete_st (decreases length l) =
+  match length l with
+  |0 -> x
+  |_ -> apply_log (do x (head l)) (tail l)                   
+
+// property of apply_log
+let rec lem_apply_log (x:concrete_st) (l:log)
+  : Lemma (ensures (length l > 0 ==> apply_log x l == do (apply_log x (fst (un_snoc l))) (last l)))
+          (decreases length l) =
+  match length l with
+  |0 -> ()
+  |_ -> lem_apply_log (do x (head l)) (tail l)
+
+#push-options "--z3rlimit 50 --ifuel 3"
+let rec lem_apply (x:concrete_st) (l:log)
+  : Lemma (ensures (let r = apply_log x l in
+                        //(forall rid. M.contains r rid ==> M.contains x rid \/ mem_rid rid l) /\
+                        (forall rid. M.contains x rid ==> M.contains r rid) /\
+                        (forall rid. fst (sel r rid) >= fst (sel x rid))))
+          (decreases length l) =
+          //[SMTPat (apply_log x l)] =
+  match length l with
+  |0 -> ()
+  |_ -> lem_apply (do x (head l)) (tail l)
+#pop-options
+
+type st1 = s:st0{(v_of s == apply_log init_st (ops_of s))}
+
+let valid_st (s:st0) : prop =
+  distinct_ops (ops_of s) /\
+  (v_of s == apply_log init_st (ops_of s))
+
+type st = s:st0{valid_st s}
 
 type resolve_conflict_res =
   | First_then_second // op2.op1 
@@ -73,6 +135,269 @@ let concrete_merge (lca s1 s2:concrete_st) : concrete_st =
   let keys = S.union (M.domain lca) (S.union (M.domain s1) (M.domain s2)) in
   let u = M.const_on keys (0, false) in
   M.iter_upd (fun k v -> merge_cf (sel lca k) (sel s1 k) (sel s2 k)) u
+
+let inverse_st (s:st{Seq.length (ops_of s) > 0}) 
+  : GTot (i:st{(v_of s == do (v_of i) (last (ops_of s))) /\
+               (ops_of i = fst (un_snoc (ops_of s))) /\
+               (ops_of s = snoc (ops_of i) (last (ops_of s))) /\
+               is_prefix (ops_of i) (ops_of s) /\
+               (forall id. mem_id id (ops_of i) <==> mem_id id (ops_of s) /\ id <> fst (last (ops_of s)))}) =
+  let p,_ = un_snoc (ops_of s) in
+  let r = apply_log init_st p in
+  lem_apply_log init_st (ops_of s);
+  let p, l = un_snoc (ops_of s) in
+  let r = apply_log init_st p in
+  lemma_split (ops_of s) (length (ops_of s) - 1); 
+  lemma_append_count_assoc_fst p (snd (split (ops_of s) (length (ops_of s) - 1))); 
+  distinct_invert_append p (snd (split (ops_of s) (length (ops_of s) - 1)));
+  (r, hide p)
+
+//currently present in App.fsti as Log MRDT needs it
+let rec inverse_helper (s:concrete_st) (l':log) (op:op_t)
+  : Lemma (ensures (let l = Seq.snoc l' op in 
+                   (apply_log s l == do (apply_log s l') op))) 
+          (decreases length l')
+  = Seq.un_snoc_snoc l' op;
+    match length l' with
+    |0 -> ()
+    |_ -> inverse_helper (do s (head l')) (tail l') op
+
+//currently present in App.fsti as Log MRDT needs it
+let rec split_prefix (s:concrete_st) (l:log) (a:log)
+  : Lemma (requires is_prefix l a)
+          (ensures (apply_log s a == apply_log (apply_log s l) (diff a l)) /\
+                   (forall e. mem e l ==> mem e a) /\
+                   (Seq.length a > Seq.length l ==> (last a) == (last (diff a l))))
+          (decreases Seq.length l)
+  = match Seq.length l with
+    |0 -> ()
+    |_ -> split_prefix (do s (head l)) (tail l) (tail a)
+
+let consistent_branches (lca s1 s2:st1) =
+  distinct_ops (ops_of lca) /\ distinct_ops (ops_of s1) /\ distinct_ops (ops_of s2) /\
+  is_prefix (ops_of lca) (ops_of s1) /\
+  is_prefix (ops_of lca) (ops_of s2) /\
+  (forall id id1. mem_id id (ops_of lca) ==> not (mem_id id1 (diff (ops_of s1) (ops_of lca)))) /\
+  (forall id id1. mem_id id (ops_of lca) ==> not (mem_id id1 (diff (ops_of s2) (ops_of lca)))) /\
+  (forall id. mem_id id (diff (ops_of s1) (ops_of lca)) ==> not (mem_id id (diff (ops_of s2) (ops_of lca)))) /\
+  (forall rid. mem_rid rid (diff (ops_of s1) (ops_of lca)) ==> ~ (mem_rid rid (diff (ops_of s2) (ops_of lca))))
+
+let consistent_branches_s1_gt0 (lca s1 s2:st1) =
+  consistent_branches lca s1 s2 /\
+  length (ops_of s1) > length (ops_of lca)
+
+let consistent_branches_s2_gt0 (lca s1 s2:st1) =
+  consistent_branches lca s1 s2 /\
+  length (ops_of s2) > length (ops_of lca)
+
+let consistent_branches_s1s2_gt0 (lca s1 s2:st1) =
+  consistent_branches lca s1 s2 /\
+  length (ops_of s1) > length (ops_of lca) /\
+  length (ops_of s2) > length (ops_of lca)
+
+let do_st (s:st1) (o:op_t) : st1 =
+  split_prefix init_st (ops_of s) (snoc (ops_of s) o); 
+  (do (v_of s) o, hide (snoc (ops_of s) o))
+
+let merge_is_comm (lca s1 s2:st)
+  : Lemma (requires true) //consistent_branches lca s1 s2)
+          (ensures (eq (concrete_merge (v_of lca) (v_of s1) (v_of s2)) 
+                       (concrete_merge (v_of lca) (v_of s2) (v_of s1)))) = ()
+
+#push-options "--z3rlimit 50 --ifuel 3"
+let linearizable_s1_0''_base_base (lca s1 s2':st) (last2:op_t)
+  : Lemma (requires //consistent_branches lca s1 (do_st s2' last2) /\
+                    ops_of s1 = ops_of lca /\ ops_of s2' = ops_of lca /\
+                    length (ops_of lca) = 0)
+        
+          (ensures eq (do (v_of s2') last2) (concrete_merge (v_of lca) (v_of s1) (do (v_of s2') last2))) = ()
+
+let linearizable_s1_0''_base_ind (lca s1 s2':st) (last2:op_t)
+  : Lemma (requires //consistent_branches lca s1 (do_st s2' last2) /\
+                    ops_of s1 = ops_of lca /\ ops_of s2' = ops_of lca /\
+                    length (ops_of lca) > 0 /\
+
+                    (let l' = inverse_st lca in
+                    let s1' = inverse_st s1 in
+                    let s2'' = inverse_st s2' in
+                    //consistent_branches l' s1' (do_st s2'' last2) /\
+                    ops_of s1' = ops_of l' /\ ops_of s2'' = ops_of l' /\
+                    eq (do (v_of s2'') last2) (concrete_merge (v_of l') (v_of s1') (do (v_of s2'') last2))))
+
+          (ensures eq (do (v_of s2') last2) (concrete_merge (v_of lca) (v_of s1) (do (v_of s2') last2))) = ()
+
+let linearizable_s1_0''_ind_help (lca s1 s2':st) (last2:op_t)
+  : Lemma (requires //consistent_branches lca s1 (do_st s2' last2) /\
+                    ops_of s1 == ops_of lca /\
+                    length (ops_of s2') > length (ops_of lca) /\
+
+                    (let inv2 = inverse_st s2' in
+                    consistent_branches lca s1 (do_st inv2 last2) /\
+                    eq (do (v_of inv2) last2) (concrete_merge (v_of lca) (v_of s1) (do (v_of inv2) last2))))
+        
+          (ensures (let inv2 = inverse_st s2' in
+                   (forall id. M.contains (v_of lca) id ==> M.contains (v_of s1) id /\ M.contains (do (v_of inv2) last2) id) /\
+                     (forall id. M.contains (concrete_merge (v_of lca) (v_of s1) (do (v_of inv2) last2)) id ==>
+                            fst (sel (v_of s1) id) >= fst (sel (v_of lca) id) /\
+                            fst (sel (do (v_of inv2) last2) id) >= fst (sel (v_of lca) id)))) = 
+  let inv2 = inverse_st s2' in
+  split_prefix init_st (ops_of lca) (ops_of (do_st inv2 last2));
+  lem_apply init_st (ops_of lca);
+  lem_apply (v_of lca) (diff (snoc (ops_of inv2) last2) (ops_of lca))
+
+let linearizable_s1_0''_ind (lca s1 s2':st) (last2:op_t)
+  : Lemma (requires //consistent_branches lca s1 (do_st s2' last2) /\
+                    ops_of s1 == ops_of lca /\
+                    length (ops_of s2') > length (ops_of lca) /\
+
+                    (let inv2 = inverse_st s2' in
+                    consistent_branches lca s1 (do_st inv2 last2) /\
+                    eq (do (v_of inv2) last2) (concrete_merge (v_of lca) (v_of s1) (do (v_of inv2) last2))))
+        
+          (ensures eq (do (v_of s2') last2) (concrete_merge (v_of lca) (v_of s1) (do (v_of s2') last2))) = 
+  linearizable_s1_0''_ind_help lca s1 s2' last2
+
+let linearizable_s1_0_s2_0_base (lca s1 s2:st)
+  : Lemma (requires //consistent_branches lca s1 s2 /\
+                    ops_of s1 == ops_of lca /\ ops_of s2 == ops_of lca)       
+          (ensures eq (v_of lca) (concrete_merge (v_of lca) (v_of s1) (v_of s2))) = ()
+
+let linearizable_gt0_base_fts (lca s1 s2:st) (last1 last2:op_t)
+  : Lemma (requires //consistent_branches lca (do_st s1 last1) (do_st s2 last2) /\
+                    //consistent_branches lca s1 s2 /\
+                    ops_of s1 = ops_of lca /\ ops_of s2 = ops_of lca /\
+                    fst last1 <> fst last2 /\
+                    First_then_second? (resolve_conflict last1 last2))
+         
+          (ensures eq (do (concrete_merge (v_of lca) (v_of s1) (do (v_of s2) last2)) last1)
+                      (concrete_merge (v_of lca) (do (v_of s1) last1) (do (v_of s2) last2))) = ()
+
+let linearizable_gt0_base_stf (lca s1 s2:st) (last1 last2:op_t)
+  : Lemma (requires //consistent_branches lca (do_st s1 last1) (do_st s2 last2) /\
+                    //consistent_branches lca s1 s2 /\
+                    ops_of s1 = ops_of lca /\ ops_of s2 = ops_of lca /\
+                    fst last1 <> fst last2 /\
+                    Second_then_first? (resolve_conflict last1 last2))
+         
+          (ensures eq (do (concrete_merge (v_of lca) (do (v_of s1) last1) (v_of s2)) last2)
+                      (concrete_merge (v_of lca) (do (v_of s1) last1) (do (v_of s2) last2))) = ()
+
+let linearizable_gt0_ind_fts (lca s1 s2:st) (last1 last2:op_t)
+  : Lemma (requires //consistent_branches lca (do_st s1 last1) (do_st s2 last2) /\
+                    //consistent_branches lca s1 s2 /\
+                    length (ops_of s2) > length (ops_of lca) /\
+                    fst last1 <> fst last2 /\
+                    (let s2' = inverse_st s2 in
+                    First_then_second? (resolve_conflict last1 last2) /\
+                    //consistent_branches lca s1 (do_st s2' last2) /\
+                    //consistent_branches lca (do_st s1 last1) (do_st s2' last2) /\
+                    //consistent_branches lca s1 (do_st s2 last2) /\
+                    eq (do (concrete_merge (v_of lca) (v_of s1) (do (v_of s2') last2)) last1)
+                       (concrete_merge (v_of lca) (do (v_of s1) last1) (do (v_of s2') last2))))
+       
+          (ensures eq (do (concrete_merge (v_of lca) (v_of s1) (do (v_of s2) last2)) last1)
+                      (concrete_merge (v_of lca) (do (v_of s1) last1) (do (v_of s2) last2))) = ()
+
+let linearizable_gt0_ind_stf (lca s1 s2:st) (last1 last2:op_t)
+  : Lemma (requires //consistent_branches lca (do_st s1 last1) (do_st s2 last2) /\
+                    //consistent_branches lca s1 s2 /\
+                    length (ops_of s2) > length (ops_of lca) /\
+                    fst last1 <> fst last2 /\
+                    (let s2' = inverse_st s2 in
+                    ops_of s1 = ops_of lca /\
+                    Second_then_first? (resolve_conflict last1 last2) /\
+                    //consistent_branches lca (do_st s1 last1) s2' /\
+                    //consistent_branches lca (do_st s1 last1) (do_st s2' last2) /\
+                    //consistent_branches lca (do_st s1 last1) s2 /\
+                    eq (do (concrete_merge (v_of lca) (do (v_of s1) last1) (v_of s2')) last2)
+                       (concrete_merge (v_of lca) (do (v_of s1) last1) (do (v_of s2') last2))))
+       
+          (ensures eq (do (concrete_merge (v_of lca) (do (v_of s1) last1) (v_of s2)) last2)
+                      (concrete_merge (v_of lca) (do (v_of s1) last1) (do (v_of s2) last2))) = ()
+
+let linearizable_gt0_ind1_fts (lca s1 s2:st) (last1 last2:op_t)
+  : Lemma (requires //consistent_branches lca (do_st s1 last1) (do_st s2 last2) /\
+                    //consistent_branches lca s1 s2 /\
+                    length (ops_of s1) > length (ops_of lca) /\
+                    fst last1 <> fst last2 /\
+                    (let s1' = inverse_st s1 in
+                    ops_of s2 = ops_of lca /\
+                    First_then_second? (resolve_conflict last1 last2) /\
+                    //consistent_branches lca s1' (do_st s2 last2) /\
+                    //consistent_branches lca (do_st s1' last1) (do_st s2 last2) /\
+                    //consistent_branches lca s1 (do_st s2 last2) /\
+                    eq (do (concrete_merge (v_of lca) (v_of s1') (do (v_of s2) last2)) last1)
+                       (concrete_merge (v_of lca) (do (v_of s1') last1) (do (v_of s2) last2))))
+                           
+          (ensures eq (do (concrete_merge (v_of lca) (v_of s1) (do (v_of s2) last2)) last1)
+                      (concrete_merge (v_of lca) (do (v_of s1) last1) (do (v_of s2) last2))) = ()
+
+let linearizable_gt0_ind1_stf_de (lca s1 s2:st) (last1 last2:op_t)
+  : Lemma (requires //consistent_branches lca (do_st s1 last1) (do_st s2 last2) /\
+                    //consistent_branches lca s1 s2 /\
+                    length (ops_of s1) > length (ops_of lca) /\
+                    fst last1 <> fst last2 /\
+                    Disable? (snd (snd last1)) /\ Enable? (snd (snd last2)) /\
+                    (let s1' = inverse_st s1 in
+                    Second_then_first? (resolve_conflict last1 last2) /\
+                    //consistent_branches lca (do_st s1' last1) s2 /\
+                    //consistent_branches lca (do_st s1' last1) (do_st s2 last2) /\
+                    //consistent_branches lca (do_st s1 last1) s2 /\
+                    eq (do (concrete_merge (v_of lca) (do (v_of s1') last1) (v_of s2)) last2)
+                       (concrete_merge (v_of lca) (do (v_of s1') last1) (do (v_of s2) last2))))
+                           
+          (ensures eq (do (concrete_merge (v_of lca) (do (v_of s1) last1) (v_of s2)) last2)
+                      (concrete_merge (v_of lca) (do (v_of s1) last1) (do (v_of s2) last2))) = ()
+
+let linearizable_gt0_ind1_stf_dd (lca s1 s2:st) (last1 last2:op_t)
+  : Lemma (requires //consistent_branches lca (do_st s1 last1) (do_st s2 last2) /\
+                    //consistent_branches lca s1 s2 /\
+                    length (ops_of s1) > length (ops_of lca) /\
+                    fst last1 <> fst last2 /\
+                    Disable? (snd (snd last1)) /\ Disable? (snd (snd last2)) /\
+                    (let s1' = inverse_st s1 in
+                    Second_then_first? (resolve_conflict last1 last2) /\
+                    //consistent_branches lca (do_st s1' last1) s2 /\
+                    //consistent_branches lca (do_st s1' last1) (do_st s2 last2) /\
+                    //consistent_branches lca (do_st s1 last1) s2 /\
+                    eq (do (concrete_merge (v_of lca) (do (v_of s1') last1) (v_of s2)) last2)
+                       (concrete_merge (v_of lca) (do (v_of s1') last1) (do (v_of s2) last2))))
+                           
+          (ensures eq (do (concrete_merge (v_of lca) (do (v_of s1) last1) (v_of s2)) last2)
+                      (concrete_merge (v_of lca) (do (v_of s1) last1) (do (v_of s2) last2))) = ()
+
+let linearizable_gt0_ind1_stf_ee_help (lca s1 s2:st) (last1 last2:op_t)
+  : Lemma (requires consistent_branches lca (do_st s1 last1) (do_st s2 last2) /\
+                    consistent_branches lca s1 s2)
+          (ensures (forall id. M.contains (v_of lca) id ==> M.contains (do (v_of s1) last1) id /\  M.contains (v_of s2) id) /\
+                   (forall id. M.contains (concrete_merge (v_of lca) (do (v_of s1) last1) (v_of s2)) id ==>
+                      fst (sel (do (v_of s1) last1) id) >= fst (sel (v_of lca) id) /\
+                      fst (sel (v_of s2) id) >= fst (sel (v_of lca) id))) =
+  lem_apply init_st (ops_of lca);  
+  split_prefix init_st (ops_of lca) (ops_of s2);
+  lem_apply (v_of lca) (diff (ops_of s2) (ops_of lca));
+  split_prefix init_st (ops_of lca) (ops_of (do_st s1 last1));
+  lem_apply (v_of lca) (diff (snoc (ops_of s1) last1) (ops_of lca))
+
+#push-options "--z3rlimit 100"
+let linearizable_gt0_ind1_stf_ee (lca s1 s2:st) (last1 last2:op_t)
+  : Lemma (requires consistent_branches lca (do_st s1 last1) (do_st s2 last2) /\
+                    consistent_branches lca s1 s2 /\
+                    length (ops_of s1) > length (ops_of lca) /\
+                    fst last1 <> fst last2 /\
+                    Enable? (snd (snd last1)) /\ Enable? (snd (snd last2)) /\
+                    (let s1' = inverse_st s1 in
+                    Second_then_first? (resolve_conflict last1 last2) /\
+                    //consistent_branches lca (do_st s1' last1) s2 /\
+                    //consistent_branches lca (do_st s1' last1) (do_st s2 last2) /\
+                    //consistent_branches lca (do_st s1 last1) s2 /\
+                    eq (do (concrete_merge (v_of lca) (do (v_of s1') last1) (v_of s2)) last2)
+                       (concrete_merge (v_of lca) (do (v_of s1') last1) (do (v_of s2) last2))))
+                           
+          (ensures eq (do (concrete_merge (v_of lca) (do (v_of s1) last1) (v_of s2)) last2)
+                      (concrete_merge (v_of lca) (do (v_of s1) last1) (do (v_of s2) last2))) = 
+  linearizable_gt0_ind1_stf_ee_help lca s1 s2 last1 last2
+#push-options
 
 ////////////////////////////////////////////////////////////////
 //// Linearization properties - intermediate merge //////
